src/probability/iterateScript.sml
@@ -20,9 +20,9 @@
 open HolKernel Parse boolLib bossLib;
 
 open numLib unwindLib tautLib Arith
-prim_recTheory combinTheory quotientTheory arithmeticTheory hrealTheory
+prim_recTheory combinTheory quotientTheory arithmeticTheory
 realaxTheory realTheory realLib jrhUtils pairTheory seqTheory limTheory
-transcTheory listTheory mesonLib boolTheory pred_setTheory pred_setLib
+transcTheory listTheory mesonLib boolTheory pred_setTheory
 optionTheory numTheory sumTheory InductiveDefinition ind_typeTheory;
 
 open wellorderTheory cardinalTheory hurdUtils;
@@ -35,8 +35,6 @@ val _ = new_theory "iterate";
 
 fun MESON ths tm = prove(tm,MESON_TAC ths);
 fun METIS ths tm = prove(tm,METIS_TAC ths);
-
-val SET_RULE = SET_CONV; (* for backward compatibility *)
 
 val DISC_RW_KILL = DISCH_TAC THEN ONCE_ASM_REWRITE_TAC [] THEN
                    POP_ASSUM K_TAC;
