README.md
@@ -1,2 +1,31 @@
-# HOL-Probability
-The new [0,+inf]-measure and probability theory for HOL4 (ongoing work)
+# HOL's Probability Theory
+
+This directory contains HOL4's Measure, Lebesgue integral and Probability theories.
+
+## Preliminaries
+
+     sigma_algebraScript.sml      * Sigma algebra and other system of sets
+     extrealScript.sml            * The theory of Extended Real Numbers
+     real_topologyScript.sml      * Elementary Topology in Euclidean Space (from HOL Light)
+
+## Measure, Integral and Probability Theory defined on extended reals (new)
+
+     measureScript.sml            * Measure Theory defined on extended reals
+     borelScript.sml              * Borel sets and Borel measurable functions
+     lebesgueScript.sml           * The theory of Lebesgue Integral
+     martingaleScript.sml         * The theory of martingales based on σ-finite filtered measure space
+     probabilityScript.sml        * Probability Theory based on extended reals
+
+## Measure, Integral and Probability Theory defined on reals (old)
+
+     real_measureScript.sml       * Measure Theory defined on reals
+     real_borelScript.sml         * Borel measurable sets generated from reals
+     real_lebesgueScript.sml      * The theory of Lebesgue Integral based on reals
+     real_probabilityScript.sml   * Probability Theory based on reals
+
+## Utilities
+
+     hurdUtils.{sml|sig}          * Some useful tools originally defined by Joe Hurd
+     util_probScript.sml          * Utility lemmas needed by other scripts
+     iterateScript.sml            * Generic iterated operations and special cases of sums over N and R
+     productScript.sml            * Products of natural numbers and real numbers
